Fix an SMTPat in FStar.Sequence

ulib/FStar.Seq.Base.fst
@@ -246,10 +246,9 @@ abstract let append_empty_r
 
 
 abstract
-val init_index (#a:Type) (len:nat) (contents:(i:nat { i < len } -> Tot a))
+val init_index_ (#a:Type) (len:nat) (contents:(i:nat { i < len } -> Tot a))
   : Lemma (requires True)
     (ensures (forall (i:nat{i < len}). index (init len contents) i == contents i))
-    [SMTPat (index (init len contents))]
 
 private
 let rec init_index_aux (#a:Type) (len:nat) (k:nat{k < len}) (contents:(i:nat { i < len } -> Tot a))
@@ -266,8 +265,14 @@ let rec init_index_aux (#a:Type) (len:nat) (k:nat{k < len}) (contents:(i:nat { i
       else index (init_aux len k contents) i == index (init_aux len (k+1) contents) (i-1))
   end
 
-let init_index #a len contents =
+let init_index_ #a len contents =
   if len = 0 then () else init_index_aux #a len 0 contents
+
+abstract
+val init_index (#a:Type) (len:nat) (contents:(i:nat { i < len } -> Tot a)) (j: nat)
+  : Lemma (requires j < len)
+    (ensures (index (init len contents) j == contents j))
+    [SMTPat (index (init len contents) j)]
 
 let lemma_equal_instances_implies_equal_types ()
   :Lemma (forall (a:Type) (b:Type) (s1:seq a) (s2:seq b). s1 === s2 ==> a == b)
